BoogieLang/BoogieDeBruijn.thy
@@ -13,7 +13,7 @@ where
   "shiftT n k (TVar i) = (if i < k then TVar i else TVar (i + n))"
 | "shiftT n k (TPrim tp) = (TPrim tp)"
 | "shiftT n k (TCon tcon_id ty_args) = (TCon tcon_id (map (shiftT n k) ty_args))"
-| "shiftT n k (TMap ty_keys ty_val) = (TMap (map (shiftT n k) ty_keys) (shiftT n k ty_val))"
+| "shiftT n k (TMap ty_key ty_val) = (TMap ((shiftT n k) ty_key) (shiftT n k ty_val))"
 
 primrec shift :: "nat \<Rightarrow> nat \<Rightarrow> expr \<Rightarrow> expr" ("\<up>")
 where
@@ -23,6 +23,8 @@ where
 | "\<up> n k (UnOp uop e) = UnOp uop (\<up> n k e)"
 | "\<up> n k (e1 \<guillemotleft>bop\<guillemotright> e2) = (\<up> n k e1) \<guillemotleft>bop\<guillemotright> (\<up> n k e2)"
 | "\<up> n k (FunExp f ty_args args) = FunExp f ty_args (map (\<up> n k) args)"
+| "\<up> n k (MapSelect m key) = MapSelect (\<up> n k m) (\<up> n k key)"
+| "\<up> n k (MapStore m key val) = MapStore (\<up> n k m) (\<up> n k key) (\<up> n k val)"
 | "\<up> n k (CondExp cond els thn) = CondExp (\<up> n k cond) (\<up> n k els) (\<up> n k thn)"
 | "\<up> n k (Old e) = Old (\<up> n k e)"
 | "\<up> n k (Forall ty e) = (Forall ty (\<up> n (k+1) e))"
@@ -41,6 +43,8 @@ primrec shift_ty_term :: "nat \<Rightarrow> nat \<Rightarrow> expr \<Rightarrow>
 | "\<up>\<^sub>\<tau> n k (UnOp uop e) = UnOp uop (\<up>\<^sub>\<tau> n k e)"
 | "\<up>\<^sub>\<tau> n k (e1 \<guillemotleft>bop\<guillemotright> e2) = (\<up>\<^sub>\<tau> n k e1) \<guillemotleft>bop\<guillemotright> (\<up>\<^sub>\<tau> n k e2)"
 | "\<up>\<^sub>\<tau> n k (FunExp f ty_args args) = FunExp f (map (shiftT n k) ty_args) (map (\<up>\<^sub>\<tau> n k) args)"
+| "\<up>\<^sub>\<tau> n k (MapSelect m key) = MapSelect (\<up>\<^sub>\<tau> n k m) (\<up>\<^sub>\<tau> n k key)"
+| "\<up>\<^sub>\<tau> n k (MapStore m key val) = MapStore (\<up>\<^sub>\<tau> n k m) (\<up>\<^sub>\<tau> n k key) (\<up>\<^sub>\<tau> n k val)"
 | "\<up>\<^sub>\<tau> n k (CondExp cond thn els) = CondExp (\<up>\<^sub>\<tau> n k cond) (\<up>\<^sub>\<tau> n k thn) (\<up>\<^sub>\<tau> n k els)"
 | "\<up>\<^sub>\<tau> n k (Old e) = Old (\<up>\<^sub>\<tau> n k e)"
 | "\<up>\<^sub>\<tau> n k (Forall ty e) = (Forall (shiftT n k ty) (\<up>\<^sub>\<tau> n k e))"
@@ -54,7 +58,7 @@ primrec substT :: "ty \<Rightarrow> nat \<Rightarrow> ty \<Rightarrow> ty"  ("_[
   "(TVar i)[k \<mapsto>\<^sub>\<tau> S]\<^sub>\<tau> = (if k < i then TVar (i - 1) else if i = k then shiftT k 0 S else TVar i)"
 | "(TPrim p)[k \<mapsto>\<^sub>\<tau> S]\<^sub>\<tau> = TPrim p"
 | "(TCon tcon_id ty_args)[k \<mapsto>\<^sub>\<tau> S]\<^sub>\<tau> = TCon tcon_id (map (\<lambda>t. t[k \<mapsto>\<^sub>\<tau> S]\<^sub>\<tau>) ty_args)"
-| "(TMap ty_keys ty_val)[k \<mapsto>\<^sub>\<tau> S]\<^sub>\<tau> = (TMap (map (\<lambda>t. t[k \<mapsto>\<^sub>\<tau> S]\<^sub>\<tau>) ty_keys) (ty_val[k \<mapsto>\<^sub>\<tau> S]\<^sub>\<tau>))"
+| "(TMap ty_key ty_val)[k \<mapsto>\<^sub>\<tau> S]\<^sub>\<tau> = (TMap ((\<lambda>t. t[k \<mapsto>\<^sub>\<tau> S]\<^sub>\<tau>) ty_key) (ty_val[k \<mapsto>\<^sub>\<tau> S]\<^sub>\<tau>))"
 
 text\<open>At the top-level, e[k \<mapsto>_\<tau> S] must only be used for k = 0, since the function assumes that
 S must be shifted by j if variable j must be substituted.\<close>
@@ -67,6 +71,8 @@ primrec subst_ty_expr :: "expr \<Rightarrow> nat \<Rightarrow> ty \<Rightarrow> 
   | "(UnOp uop e)[k \<mapsto>\<^sub>\<tau> S] = UnOp uop (e[k \<mapsto>\<^sub>\<tau> S])"
   | "(e1 \<guillemotleft>bop\<guillemotright> e2)[k \<mapsto>\<^sub>\<tau> S] = (e1[k \<mapsto>\<^sub>\<tau> S]) \<guillemotleft>bop\<guillemotright> (e2[k \<mapsto>\<^sub>\<tau> S])"
   | "(FunExp f ty_args args)[k \<mapsto>\<^sub>\<tau> S] = FunExp f (map (\<lambda>t. t[k \<mapsto>\<^sub>\<tau> S]\<^sub>\<tau>) ty_args) (map (\<lambda>e. e[k \<mapsto>\<^sub>\<tau> S]) args)"
+  | "(MapSelect m key)[k \<mapsto>\<^sub>\<tau> S] = MapSelect (m[k \<mapsto>\<^sub>\<tau> S]) (key[k \<mapsto>\<^sub>\<tau> S])"
+  | "(MapStore m key val)[k \<mapsto>\<^sub>\<tau> S] = MapStore (m[k \<mapsto>\<^sub>\<tau> S]) (key[k \<mapsto>\<^sub>\<tau> S]) (val[k \<mapsto>\<^sub>\<tau> S])"
   | "(CondExp cond thn els)[k \<mapsto>\<^sub>\<tau> S] = CondExp (cond[k \<mapsto>\<^sub>\<tau> S]) (thn[k \<mapsto>\<^sub>\<tau> S]) (els[k \<mapsto>\<^sub>\<tau> S])"
   | "(Old e)[k \<mapsto>\<^sub>\<tau> S] = Old (e[k \<mapsto>\<^sub>\<tau> S])"
   | "(Forall ty e)[k \<mapsto>\<^sub>\<tau> S] = (Forall (ty[k \<mapsto>\<^sub>\<tau> S]\<^sub>\<tau>) (e[k \<mapsto>\<^sub>\<tau> S]))"
@@ -95,7 +101,7 @@ lemma shiftT_shiftT' [simp]:
 
 lemma shiftT_size [simp]: "size (shiftT n k T) = size T"
   apply (induct T arbitrary: k; simp) 
-  by sorry (* (simp add: eq_iff size_list_pointwise)*)
+  by (simp add: eq_iff size_list_pointwise)
 
 lemma shiftT0 [simp]: "shiftT 0 i T = T"
   apply (induct T arbitrary: i) by (auto simp add: map_idI)
@@ -167,7 +173,7 @@ primrec msubstT_opt_aux :: "(nat \<Rightarrow> ty option) \<Rightarrow> ty \<Rig
   "msubstT_opt_aux \<sigma> (TVar i) n = (if \<sigma> i \<noteq> None then shiftT n 0 (the (\<sigma> i)) else TVar i)"
 | "msubstT_opt_aux \<sigma> (TPrim p) n = TPrim p"
 | "msubstT_opt_aux \<sigma> (TCon tcon_id ty_args) n = TCon tcon_id (map (\<lambda>t. msubstT_opt_aux \<sigma> t n) ty_args)"
-| "msubstT_opt_aux \<sigma>  (TMap ty_keys ty_val) n = (TMap (map (\<lambda>t. msubstT_opt_aux \<sigma> t n) ty_keys) (msubstT_opt_aux \<sigma> ty_val n))"
+| "msubstT_opt_aux \<sigma> (TMap ty_key ty_val) n = (TMap ((\<lambda>t. msubstT_opt_aux \<sigma> t n) ty_key) (msubstT_opt_aux \<sigma> ty_val n))"
 
 definition msubstT_opt :: "ty list \<Rightarrow> ty \<Rightarrow> ty"
   where
